Various fstar core additions, mostly for iterators.

proof-libs/fstar/core/Core.Iter.Traits.Collect.fst
@@ -1,14 +1,39 @@
 module Core.Iter.Traits.Collect
 
-class into_iterator self = {
+open Rust_primitives
+
+class t_IntoIterator self = {
   f_IntoIter: Type0;
   // f_Item: Type0;
   f_into_iter: self -> f_IntoIter;
 }
 
-let t_IntoIterator = into_iterator
-
-unfold instance impl t {| Core.Iter.Traits.Iterator.iterator t |}: into_iterator t = {
+unfold instance impl t {| Core.Iter.Traits.Iterator.t_Iterator t |}: t_IntoIterator t = {
   f_IntoIter = t;
   f_into_iter = id;
 }
+
+class t_Extend
+  (v_Self: Type0) (v_A: Type0)
+  = {
+  f_extend_post:
+      #v_T: Type0 ->
+      {| i1:
+          Core.Iter.Traits.Collect.t_IntoIterator
+          v_T |} ->
+      v_Self ->
+      v_T ->
+      v_Self
+    -> Type0; 
+  f_extend:
+      #v_T: Type0 ->
+      {| i1:
+          Core.Iter.Traits.Collect.t_IntoIterator
+          v_T |} ->
+      x0: v_Self ->
+      x1: v_T
+    -> v_Self
+}
+
+[@@ FStar.Tactics.Typeclasses.tcinstance]
+assume val extend_slice (t: eqtype): t_Extend (t_Slice t) t
